LeanTra.lean
@@ -6,8 +6,8 @@ import LeanTra.SRA.Howe
 import LeanTra.SRA.Modality
 import LeanTra.SRA.OperationalDecomposition
 import LeanTra.Metatheory.GentzenPrinciples
-import LeanTra.Metatheory.Evaluation
-import LeanTra.Metatheory.Determinism
+import LeanTra.Metatheory.Determinism.Evaluation
+import LeanTra.Metatheory.Determinism.BigStep
 import LeanTra.Metatheory.Confluence.ParallelReduction
 import LeanTra.Metatheory.Confluence.Orthogonal
 import LeanTra.Metatheory.Confluence.Local
